policies/PVI.v
@@ -29,7 +29,7 @@ Module PVI <: Policy.
   Theorem lt_eq_dec : forall (t1 t2:loc_tag), {t1 = t2} + {t1 <> t2}.
   Proof. repeat decide equality. Qed.
 
-  Definition def_tag : val_tag := N.
+  Definition TempT   : val_tag := N.
   Definition InitPCT : control_tag := O.
   Definition DefLT   : loc_tag := N.
   Definition DefHT   : loc_tag := N.
@@ -93,7 +93,7 @@ Module PVI <: Policy.
     | _, _ => ret (pct, vt2)
     end.
 
-  Definition ConstT (l:loc) (pct : control_tag) : PolicyResult val_tag := ret N.
+  Definition LiteralT (l:loc) (pct : control_tag) : PolicyResult val_tag := ret N.
 
   Definition GlobalT (ce : composite_env) (id : ident) (ty : type) : val_tag * val_tag * loc_tag :=
     (Glob id, N, Glob id).
@@ -130,7 +130,7 @@ Module PVI <: Policy.
   Definition AccessT    := Passthrough.AccessT policy_state val_tag control_tag.
   Definition AssignT    := Passthrough.AssignT policy_state val_tag control_tag.
   Definition CoalesceT  := Passthrough.CoalesceT policy_state val_tag vt_eq_dec.
-  Definition EffectiveT := Passthrough.EffectiveT val_tag def_tag. 
+  Definition EffectiveT := Passthrough.EffectiveT val_tag TempT. 
   Definition UnopT      := Passthrough.UnopT policy_state val_tag control_tag.
   Definition SplitT     := Passthrough.SplitT policy_state val_tag control_tag.
   Definition LabelT     := Passthrough.LabelT policy_state control_tag.
@@ -138,8 +138,6 @@ Module PVI <: Policy.
   Definition ExprJoinT  := Passthrough.ExprJoinT policy_state val_tag control_tag.
   Definition FieldT     := Passthrough.FieldT policy_state val_tag control_tag.
   Definition ExtCallT   := Passthrough.ExtCallT policy_state val_tag control_tag.
-  Definition PICastT    := Passthrough.PICastT policy_state val_tag control_tag loc_tag.
-  Definition IPCastT    := Passthrough.IPCastT policy_state val_tag control_tag loc_tag.
-  Definition PPCastT    := Passthrough.PPCastT policy_state val_tag control_tag loc_tag.
-  Definition IICastT    := Passthrough.IICastT policy_state val_tag control_tag.
+  Definition CastToPtrT := Passthrough.CastToPtrT policy_state val_tag control_tag loc_tag.
+  Definition CastOtherT := Passthrough.CastOtherT policy_state val_tag control_tag.
 End PVI.
